


\documentclass{article}
\usepackage{amsmath}
\begin{document}

Given:
\begin{itemize}
    \item Cost function: \(c_0 = (a^{(L)} - y)^2\)
    \item Weighted input: \(z^{(L)} = w^{(L)} a^{(L-1)} + b^{(L)}\)
    \item Activation: \(a^{(L)} = \sigma(z^{(L)})\)
\end{itemize}

Using the chain rule to find \(\frac{\partial c_0}{\partial w^{(L)}}\):

\[
\frac{\partial c_0}{\partial w^{(L)}} = \frac{\partial c_0}{\partial a^{(L)}} \cdot \frac{\partial a^{(L)}}{\partial z^{(L)}} \cdot \frac{\partial z^{(L)}}{\partial w^{(L)}}
\]

Where:
\begin{align*}
    \frac{\partial c_0}{\partial a^{(L)}} &= 2(a^{(L)} - y) \\
    \frac{\partial a^{(L)}}{\partial z^{(L)}} &= \sigma(z^{(L)}) \cdot (1 - \sigma(z^{(L)})) \\
    \frac{\partial z^{(L)}}{\partial w^{(L)}} &= a^{(L-1)}
\end{align*}


So the weights are:
\begin{align*}
    \frac{\partial c_0}{\partial w^{(L)}} &= a^{(L-1)} \cdot \partiel \sigma(z^{(L)}) \cdot 2(a^{(L)} - y)
\end{align*}

The bias is:
\begin{align*}
    \frac{\partial c_0}{\partial b^{(L)}} &= \partiel \sigma(z^{(L)}) \cdot 2(a^{(L)} - y)
\end{align*}

\end{document}
